src/project/task_change.rs
@@ -103,6 +103,7 @@ fn batch_operation(operation: task::AuthorOperation) -> author::BatchOperation {
     match operation {
         task::AuthorOperation::ReplaceBody => author::BatchOperation::ReplaceBody,
         task::AuthorOperation::ReplaceBodySemantic => author::BatchOperation::ReplaceBodySemantic,
+        task::AuthorOperation::EditBodySemantic => author::BatchOperation::EditBodySemantic,
         task::AuthorOperation::ReplaceDeclaration => author::BatchOperation::ReplaceDeclaration,
         task::AuthorOperation::InsertDeclaration => author::BatchOperation::InsertDeclaration,
         task::AuthorOperation::OrganizeImports => author::BatchOperation::OrganizeImports,
